Environment.v
@@ -1,0 +1,116 @@
+Require Import Arith List.
+
+Inductive environment A :=
+| Empty : environment A
+| Extend : nat -> A -> environment A -> environment A.
+
+Fixpoint lookup {A : Type} x env : option A :=
+  match env with
+    | Empty =>
+      None
+    | Extend x' a env' =>
+      if beq_nat x x'
+      then Some a
+      else lookup x env'
+  end.
+
+Definition env_equiv {A : Type} env  env' :=
+  forall x,
+    @lookup A x env = lookup x env'.
+
+Require Import Setoid.
+
+Instance tc_env_equiv {A : Type} : Equivalence (@env_equiv A).
+Proof.
+  unfold env_equiv.
+  split.
+  unfold Reflexive; intros.
+  reflexivity.
+  unfold Symmetric; intros.
+  rewrite H.
+  reflexivity.
+  unfold Transitive; intros.
+  rewrite H, H0.
+  reflexivity.
+Qed.
+
+Lemma env_equiv_extend_eq {A : Type} :
+  forall x v env env',
+    env_equiv env env' ->
+    env_equiv (Extend A x v env) (Extend A x v env').
+Proof.
+  unfold env_equiv.
+  intros.
+  simpl.
+  destruct (beq_nat x0 x).
+  reflexivity.
+  apply H.
+Qed.
+
+Lemma lookup_empty {A : Type} :
+  forall x,
+    lookup x (Empty A) = None.
+Proof.
+  reflexivity.
+Qed.
+
+Lemma lookup_extend_eq {A : Type} :
+  forall x v env,
+    lookup x (Extend A x v env) = Some v.
+Proof.
+  intros.
+  simpl.
+  rewrite <- beq_nat_refl.
+  reflexivity.
+Qed.
+
+Lemma lookup_extend_neq {A : Type} :
+  forall x x' v' env,
+    beq_nat x x' = false ->
+    lookup x (Extend A x' v' env) = lookup x env.
+Proof.
+  intros.
+  simpl.
+  rewrite H.
+  reflexivity.
+Qed.
+
+Lemma env_shadow :
+  forall A x v v' env,
+    env_equiv (Extend A x v (Extend A x v' env)) (Extend A x v env).
+Proof.
+  intros.
+  unfold env_equiv.
+  intros x'.
+  simpl.
+  remember (beq_nat x' x) as b.
+  destruct b.
+  reflexivity.
+  reflexivity.
+Qed.
+
+Lemma env_permute :
+  forall A x x' v v' env,
+    beq_nat x x' = false ->
+    env_equiv (Extend A x v (Extend A x' v' env)) (Extend A x' v' (Extend A x v env)).
+Proof.
+  intros.
+  unfold env_equiv.
+  intros y.
+  simpl.
+  remember (beq_nat y x) as eqyx.
+  destruct eqyx.
+  symmetry in Heqeqyx.
+  apply beq_nat_true in Heqeqyx.
+  rewrite Heqeqyx.
+  rewrite H.
+  reflexivity.
+  reflexivity.
+Qed.
+
+Definition distinct {A : Type} (env : environment A) :=
+  forall x v,
+    lookup x env = Some v ->
+    exists env',
+      env_equiv (Extend A x v env') env /\
+      lookup x env' = None.
